compcertox/CModule.v
@@ -448,7 +448,7 @@ Section XXX.
     unfold comp_r.
     generalize (@eq_refl (option B) (comp_b (R_b r1) (R_b r2))).
     generalize (comp_b (R_b r1) (R_b r2)) at 1 3.
-    intros [o|].
+    intros [x|].
     - intros H X. inv X. reflexivity.
     - intros H X. inv X.
   Qed.
